\documentclass[]{article}
\usepackage{subfiles}
\usepackage{hyperref}
\usepackage{csquotes}
\usepackage{amsmath}
\usepackage{amsfonts}
\usepackage[]{geometry}
\usepackage{graphicx}
\usepackage{listings}
\usepackage{xcolor}

\begin{document}
    \section[P4: Simplified \texorpdfstring{$\sigma^2$}{variance}]{Simplified variance for discrete random variables}
    Reiterating the equation which has to be proven
    \begin{equation}
        Var(X) = Cov(X, X) = E \left [ \left (X - E[X] \right )^2 \right ] = E[X^2] - \left ( E[X] \right )^2
        \tag{\ref{eq:var} revisited}
        \label{eq:var-2}
    \end{equation}
    Starting from the left side of \ref{eq:var-2}, we get
    \begin{equation}
        \label{eq:p4-to-prove}
        Var(X) = Cov(X, X) = E \left [ \left (X - E[X] \right )^2 \right ]
    \end{equation}
    The expectation for a function of a discrete random variable $X$ (whose possible values are given by $R_X$), is given by
    \begin{equation}
        E_{x \sim X} \left [ f(X) \right ] = \sum_{x \in R_X} f(x) P(X=x)
    \end{equation}
    Simplifying the equation \ref{eq:p4-to-prove} using the following known conditions
    \begin{enumerate}
        \item The value of $E[X]$ is the mean of the discrete random variable given by \\
            \begin{equation}
                E[X] = \sum_{x \in R_X} x P_X(x) = \mu
            \end{equation}
        \item $\mu$ is a constant for a given probability distribution $P_X$
        \item $\sum_{x \in R_X} P_X(x) = 1$ because $P_X$ is a probability mass function
    \end{enumerate}
    we get
    \begin{equation}
        \label{eq:p4-var-proof}
        \begin{split}
            E \left [ \left (X - E[X] \right )^2 \right ] & = E \left [ \left (X - \mu \right )^2 \right ]
            = \sum_{x \in R_X} \left ( x - \mu \right )^2 P_X(x)
            = \sum_{x \in R_X} \left ( x^2 + \mu^2 - 2x\mu \right ) P_X(x) \\
            & = \sum_{x \in R_X} x^2 P_X(x) + \mu^2 \sum_{x \in R_X} P_X(x) - 2\mu \sum_{x \in R_X} x P_X(x) \\
            & = E_{x\sim X}[X^2] + \mu^2 \cdot 1 - 2\mu \cdot \mu = E[X^2] + \mu^2 - 2\mu^2 = E[X^2] - \mu^2 \\
            & = E[X^2] - \left ( E[X] \right )^2
        \end{split}
    \end{equation}
    The equation \ref{eq:p4-var-proof} proves \ref{eq:var-2}, we therefore obtain
    \begin{equation}
        Var(X) = E[X^2] - \left ( E[X] \right )^2
    \end{equation}
\end{document}
